src/PlutusIR/Semantics/Static/Min_Ex_Subst.v
@@ -1,0 +1,188 @@
+From Equations Require Import Equations.
+Require Import Coq.Strings.String.
+Require Import Coq.Lists.List.
+Require Import Coq.micromega.Lia.
+Import ListNotations.
+Open Scope string_scope.
+Open Scope list_scope.
+
+(** kinds *)
+Inductive kind :=
+  | Kind_Base : kind
+  | Kind_Arrow : kind -> kind -> kind.
+
+(** Types *)
+Inductive ty :=
+  | Var : string -> ty
+  | Lam : string -> kind -> ty -> ty
+  | App : ty -> ty -> ty.
+
+(** Values *)
+Inductive value : ty -> Prop :=
+| v_neutral : forall ty1,
+    neutral ty1 ->
+    value ty1
+| v_abs : forall x K2 ty1,
+    value ty1 ->
+    value (Lam x K2 ty1)
+    
+    with neutral : ty -> Prop :=
+    | ne_var : forall x,
+        neutral (Var x)
+    | ne_app : forall ty1 ty2,
+        neutral ty1 ->
+        value ty2 ->
+        neutral (App ty1 ty2).
+
+(** Subst *)
+Fixpoint subst (X : string) (U T : ty) : ty :=
+  match T with
+  | Var Y =>
+    if X =? Y then U else Var Y
+  | Lam Y K1 T' =>
+    if X =? Y then Lam Y K1 T' else Lam Y K1 (subst X U T')
+  | App T1 T2 =>
+    App (subst X U T1) (subst X U T2)
+  end.
+
+(** Capture avoiding substitution*)
+Definition rename (X Y : string) (T : ty) := subst X (Var Y) T.
+
+Fixpoint size (T : ty) : nat :=
+  match T with
+  | Var Y => 1
+  | Lam bX K T0 => 1 + size T0
+  | App T1 T2 => 1 + size T1 + size T2
+  end.
+
+Fixpoint ftv (T : ty) : list string :=
+match T with
+| Var X =>
+    [X]
+| Lam X K1 T' =>
+    remove string_dec X (ftv T')
+| App T1 T2 =>
+    ftv T1 ++ ftv T2
+end.
+
+Definition fresh (X : string) (U T : ty) : string :=
+  "a" ++ X ++ (String.concat "" (ftv U)) ++ (String.concat "" (ftv T)).
+
+Lemma fresh__X : forall X U T,
+    X <> fresh X U T.
+Proof with eauto.
+  intros. intros Hcon.
+  induction X; induction (ftv U); induction (ftv T).
+  all: simpl in Hcon.
+  all: inversion Hcon; subst...
+Qed.
+
+Lemma fresh__S : forall X U T,
+    ~ In (fresh X U T) (ftv U).
+Proof. Abort.
+
+Lemma fresh__T : forall X U T,
+    ~ In (fresh X U T) (ftv T).
+Proof. Abort.
+
+Lemma rename_preserves_size : forall T X Y,
+    size T = size (rename X Y T).
+Proof.
+  unfold rename.
+  induction T; intros; simpl; eauto.
+  - destruct (X =? s); eauto.
+  - destruct (X =? s); simpl; eauto.
+Qed.
+
+Equations? substTCA (X : string) (U T : ty) : ty by wf (size T) :=
+  substTCA X U (Var Y) =>
+      if X =? Y then U else Var Y ;
+  substTCA X U (Lam Y K T) =>
+      if X =? Y
+        then
+          Lam Y K T
+        else
+          if existsb (eqb Y) (ftv U)
+            then
+              let Y' := fresh X U T in
+              let T' := rename Y Y' T in
+              Lam Y' K (substTCA X U T')
+            else
+              Lam Y K (substTCA X U T) ;
+  substTCA X U (App T1 T2) =>
+      App (substTCA X U T1) (substTCA X U T2)
+  .
+Proof.
+  all: try solve
+    [ lia
+    || replace T' with (rename Y Y' T); eauto; rewrite <- rename_preserves_size; eauto
+    ].
+Qed.
+
+(** Notation *)
+Declare Custom Entry stlc.
+Notation "<{ e }>" := e (e custom stlc at level 99).
+Notation "( x )" := x (in custom stlc, x at level 99).
+Notation "x" := x (in custom stlc at level 0, x constr at level 0).
+Notation "x y" := (App x y) (in custom stlc at level 1, left associativity).
+Notation "\ x : k , y" :=
+  (Lam x k y) (in custom stlc at level 90, x at level 99,
+                     k custom stlc at level 99,
+                     y custom stlc at level 99,
+                     left associativity).
+Reserved Notation "'[' x ':=' s ']' t" (in custom stlc at level 20, x constr).
+Notation "'[' x ':=' s ']' t" := (subst x s t) (in custom stlc).
+
+(** Step *)
+Reserved Notation "ty '-->' ty'" (at level 40).
+
+(* lambdas are no longer values unless their bodies are values*)
+(*  So we will start normalising the body*)
+Inductive step : ty -> ty -> Prop :=
+  | ST_Abs : forall ty1 ty1' x K2,
+      ty1 --> ty1' ->
+      Lam x K2 ty1 --> Lam x K2 ty1'
+  | ST_AppAbs : forall x K2 v1 v2,
+         value v1 -> (* Problematic *)
+         value v2 -> 
+         App (Lam x K2 v1) v2 --> substTCA x v2 v1
+  | ST_App1 : forall ty1 ty1' ty2,
+         ty1 --> ty1' ->
+         App ty1 ty2 --> App ty1' ty2
+  | ST_App2 : forall v1 ty2 ty2',
+         value v1 ->
+         ty2 --> ty2' ->
+         App v1 ty2 --> App v1 ty2'
+
+where "ty '-->' ty'" := (step ty ty').
+Hint Constructors step : core.
+
+(** Multistep*)
+Definition relation (X : Type) := X -> X -> Prop.
+Inductive multi {X : Type} (R : relation X) : relation X :=
+  | multi_refl : forall (x : X), multi R x x
+  | multi_step : forall (x y z : X),
+                    R x y ->
+                    multi R y z ->
+                    multi R x z.
+
+Notation multistep := (multi step).
+Notation "ty1 '-->*' ty2" := (multistep ty1 ty2) (at level 40).
+
+(** The lemma I want to prove about substitutions*)
+(* Not true:
+(* Counter example:
+   t = (\y. y) (x w) --> x w = t', 
+   then t[x=\z. v] = (\y. y) ((\z. v) w) --> (\y. y) v, 
+   while t'[x=\z. v] = (\z. v) w*)*)
+Lemma subst_preserves_step : forall X t t' v,
+  t --> t' -> value v -> subst X v t  -->* subst X v t'.
+Proof.
+  intros X t t' v H H_value_v'.
+  generalize dependent t'.
+  induction t; intros t' Hstep; inversion Hstep; eauto; subst.
+  - shelve. 
+  - rename t2 into v2. admit. (* uhm, since t2 and \x:K2,v1 are already values, IHt1 and IHt2 don't tell us anything*)
+  - shelve.
+  - shelve.
+Abort.
