src/PlutusIR/Semantics/Static/NormalisationXi.v
@@ -1,0 +1,508 @@
+From Equations Require Import Equations.
+Require Import PlutusCert.PlutusIR.
+Require Import Strings.String.
+(* Require Export PlutusCert.PlutusIR.Semantics.Static.Kinding. *)
+
+(* Require Export PlutusCert.PlutusIR.Semantics.Static.TypeSubstitution. *)
+Require Import List.
+Import ListNotations.
+From PlutusCert Require Import Analysis.FreeVars.
+Import Ty.
+Require Import Bool.
+
+Require Import Lia.
+
+Open Scope string_scope.
+
+(* Normalisation proof à la Xi and Donnelly *)
+(* Uses non-deterministic small step semantics and an implicit value definition *)
+(* For now proved for STLC with simple term language *)
+
+(** * Regular substitution of types *)
+
+Inductive tp :=
+    | tpbas : tp
+    | tpfun : tp -> tp -> tp.
+
+Inductive tps :=
+    | tpsnil : tps
+    | tpsmore : tps -> tp -> tps.
+
+Inductive tm :=
+    | tmvar : nat -> tm
+    | tmlam : tm -> tm
+    | tmapp : tm -> tm -> tm.
+
+Inductive tmshi : tm -> tm -> nat -> Prop :=
+  | TMSHIvargte : forall (i l : nat), i >= l ->
+      tmshi (tmvar i) (tmvar (i+1)) l
+  | TMSHIvarlt : forall (i l : nat), i < l ->
+      tmshi (tmvar i) (tmvar i) l
+  | TMSHIlam : forall (t t' : tm) (l : nat),
+      tmshi t t' (S l) ->
+      tmshi (tmlam t) (tmlam t') l
+  | TMSHIapp : forall (t1 t2 t1' t2' : tm) (l : nat),
+      tmshi t1 t1' l ->
+      tmshi t2 t2' l ->
+      tmshi (tmapp t1 t2) (tmapp t1' t2') l.
+
+Inductive tms :=
+  | tmsnil : tms
+  | tmsmore : tms -> tm -> tms.
+
+Inductive subshi : tms -> tms -> Prop :=
+  | SUBSHInil : subshi tmsnil tmsnil
+  | SUBSHImore : forall (ts ts' : tms) (t t' : tm),
+      subshi ts ts' ->
+      tmshi t t' 0 ->
+      subshi (tmsmore ts t) (tmsmore ts' t').
+
+Inductive TMI : nat -> tm -> tms -> Type :=
+  | TMIone : forall {ts : tms} {t : tm},
+      TMI 0 t (tmsmore ts t)
+  | TMIshi : forall {ts : tms} {t t' : tm} {i : nat}, i > 0 ->
+      TMI (i-1) t ts ->
+      TMI i t (tmsmore ts t').
+
+Inductive subst : tms -> tm -> tm -> Prop :=
+  | SUBvar : forall (ts : tms) (t : tm) (i : nat),
+      TMI i t ts ->
+      subst ts (tmvar i) t
+  | SUBlam : forall (ts ts' : tms) (t t' : tm),
+      subshi ts ts' ->
+      subst (tmsmore ts' (tmvar 0)) t t' ->
+      subst ts (tmlam t) (tmlam t')
+  | SUBapp : forall (ts : tms) (t1 t2 t1' t2' : tm),
+      subst ts t1 t1' ->
+      subst ts t2 t2' ->
+      subst ts (tmapp t1 t2) (tmapp t1' t2').
+
+Definition subst1 (t1 t2 t3 : tm) : Prop :=
+  subst (tmsmore tmsnil t1) t2 t3.
+
+Inductive TPI : nat -> tp -> tps -> Type :=
+  | TPIone : forall {G : tps} {T : tp},
+      TPI 0 T (tpsmore G T)
+  | TPIshi : forall {G : tps} {T T' : tp} {i : nat},
+      TPI i T G ->
+      TPI (S i) T (tpsmore G T').
+
+Inductive DER : tps -> tm -> tp -> nat -> Prop :=
+  | DERvar : forall (G : tps) (i : nat) (T : tp),
+      TPI i T G -> DER G (tmvar i) T 0
+
+  | DERlam : forall (G : tps) (T1 T2 : tp) (t : tm) (s : nat),
+      DER (tpsmore G T1) t T2 s ->
+      DER G (tmlam t) (tpfun T1 T2) (S s)
+
+  | DERapp : forall (G : tps) (T1 T2 : tp) (t1 t2 : tm) (s1 s2 : nat),
+      DER G t1 (tpfun T1 T2) s1 ->
+      DER G t2 T1 s2 ->
+      DER G (tmapp t1 t2) T2 (S (s1 + s2)).
+
+(* Assume the necessary definitions for tps, tm, tp, and DER are already in place *)
+
+Definition DER0 (G : tps) (t : tm) (T : tp) : Prop :=
+  exists s : nat , DER G t T s.
+
+
+
+Inductive RED : tm -> tm -> nat -> Prop :=
+  | REDlam : forall (t t' : tm) (s : nat),
+      RED t t' s ->
+      RED (tmlam t) (tmlam t') (S s)
+
+  | REDapp1 : forall (t1 t2 t1' : tm) (s : nat),
+      RED t1 t1' s ->
+      RED (tmapp t1 t2) (tmapp t1' t2) (S s)
+
+  | REDapp2 : forall (t1 t2 t2' : tm) (s : nat),
+      RED t2 t2' s ->
+      RED (tmapp t1 t2) (tmapp t1 t2') (S s)
+
+  | REDapp3 : forall (t v t' : tm),
+      subst1 v t t' -> (* Problematic. We cannot reduce (\x. x y) (3) now.*)
+      RED (tmapp (tmlam t) v) t' 0.
+
+Definition RED0 (t t' : tm) : Prop :=
+  exists s, RED t t' s.
+
+(* Implicitly says that if a term cannot reduce anymore, then it is strongly normalizing
+     (possibly with more steps (n) than absolutely necessary)*)
+(* Strong Normalization *)
+Inductive SN : tm -> nat -> Prop :=
+  | SN_intro : forall t n,
+      (forall t', RED0 t t' -> exists n', n' < n /\ SN t' n') ->
+      SN t n.
+
+Definition SN0 (t : tm) : Prop :=
+    exists n : nat, SN t n.
+
+Lemma forwardSN : forall t t' n,
+  SN t n -> RED0 t t' -> exists n', n' < n /\ SN t' n'.
+Proof.
+  intros t t' n sn red.
+  inversion sn as [t0 n0 H].
+  specialize (H t' red).
+  assumption.
+Qed.
+
+Lemma backwardSN : forall t,
+  (exists t', RED0 t t' /\ SN0 t') -> SN0 t.
+Proof.
+Admitted.
+
+(* Reducibility *)
+Fixpoint R (tm : tm) (T : tp) : Prop :=
+    match T with
+    | tpbas => SN0 tm
+    | tpfun tp1 tp2 => 
+      (forall tm', R tm' tp1 -> R (tmapp tm tm') tp2)
+    end.
+
+(* Sequence of reducibility predicates for a substitution *)
+Inductive RS : tms -> tps -> nat -> Prop :=
+  | RSnil : RS tmsnil tpsnil 0
+  | RSmore : forall {ts : tms} {t : tm} {G : tps} {T : tp} {n : nat},
+      RS ts G n ->
+      R t T ->
+      RS (tmsmore ts t) (tpsmore G T) (S n).
+
+
+
+
+
+Definition RS0 (ts : tms) (G : tps) : Type :=
+  {n : nat & RS ts G n}.
+
+(* Definition of neutral terms *)
+Inductive NEU : tm -> Type :=
+  | NEUvar : forall (i : nat), NEU (tmvar i)
+  | NEUapp : forall (t1 t2 : tm), NEU (tmapp t1 t2).
+
+Lemma mainLemmaVar : forall {G : tps} {T : tp} {ts : tms} {t : tm} {i : nat}
+  (tpi : TPI i T G) (tmi : TMI i t ts) (rs : RS0 ts G),
+  R t T.
+Proof.
+  intros G T ts t i tpi tmi rs.
+  destruct tpi as [G T | G T T' i tpi'].
+  -  (* Case: TPIone *)
+    inversion tmi.
+    + subst.
+      destruct rs as [n rs].
+      clear tmi.
+      inversion rs.
+      assumption.
+    + inversion H.
+  - inversion tmi. 
+    destruct rs as [n rs].
+    subst.
+    (* t is the S i - 1 = ith term in ts0, and T is the ith term in G, and RS ts0 G, so easy.*)
+Admitted.
+
+Require Import Coq.Arith.Arith.
+Require Import Coq.Arith.Wf_nat.
+
+(* Says: substituting x for x has no effect*)
+(* TODO: Should be provable..., but maybe changing the subst 
+    definition to capture the subst tmsnil behaviour is better*)
+Lemma vacuousSubLemma : forall {t : tm} {T : tp} {s: nat} ,
+  DER tpsnil t T s -> subst (tmsmore tmsnil (tmvar 0)) t t.
+Proof.
+  intros t T s der.
+  induction s.
+  + admit.
+  (* + apply SUBlam with (ts' := (tmsmore tmsnil (tmvar 1))). *)
+Admitted.  
+
+(* NOTE: We use inversion der instead of induction der because with induction 
+  the var case is not seen as impossible...
+  CONSEQUENCE: Now we need this s in the derivation, but we may also be able to use structural induction on der?
+  *)
+(* NOTE: In the original AST code, this did not have a well-kindedness assumption, but this is necessary for the var case*)
+Lemma lemma10 : forall {t : tm } { T : tp} {s : nat},
+  DER tpsnil t T s -> subst tmsnil t t.
+Proof.
+  (* Proof sketch:
+      DER tpsnil t T s, so no free vars in t, so it cannot be tmvar
+      For lam we get a goal like: subst (tmsmore tmsnil (tmvar 0)) t t, which says: replace (tmvar 0) by (tmvar 0), which shouldnt do anything, so true.
+
+  *)
+  intros t T s.
+  apply (well_founded_induction lt_wf (fun s => forall T, forall t, DER tpsnil t T s -> subst tmsnil t t)).
+  intros x IH.
+  intros T0 t0 der.
+  inversion der.
+  inversion der; try subst; inversion H. (* why does this not use that G=tmsnil???*)
+
+  - apply SUBlam with (ts := tmsnil) (ts' := tmsnil).
+    + apply SUBSHInil.
+    + apply vacuousSubLemma.
+      admit.
+  - apply SUBapp. (* induction lemma 10 with smaller s *)
+    + specialize (IH s1).
+      apply IH with (T := (tpfun T1 T0)).
+      * admit. (* Follows from S (s1 + s2) = x*)
+      * assumption.
+    + specialize (IH s2).
+      apply IH with (T := T1).
+      * admit. (* Follows from (S (s1 + 2))*)
+      * assumption.     
+  
+Admitted.
+
+Lemma lemma20 :
+  forall {ts ts': tms} {t t1 t' t'': tm} ,
+    subshi ts ts' ->
+    subst (tmsmore ts' (tmvar 0)) t t' ->
+    subst1 t1 t' t'' ->
+    subst (tmsmore ts t1) t t''.
+Proof.
+  intros ts ts' t t1 t' t''.
+  intros subshi sub sub1.
+  (* I thought it was impossible, but it is crucial 
+      that t' has no free variables (except for 0), this 
+      follows from inversion on subst1*)
+Admitted.
+
+
+
+(* R is preserved by forward reduction *)
+Lemma cr2 : forall (t t' : tm) (tp : tp) (n : nat),
+  R t tp -> RED0 t t' -> R t' tp.
+Proof.
+  (* intros t t' T n r rd.
+  generalize dependent t'.
+  generalize dependent t.
+  induction T; intros t r t' rd; unfold R in r; fold R in r.
+  - 
+    unfold R.
+    unfold SN0 in r.
+    destruct r as [n1 r].
+    assert (H : exists n', n' < n1 /\ SN t' n').
+    {
+      apply forwardSN with (t := t) (t' := t') (n := n1).
+      - exact r.
+      - exact rd.
+    }
+    destruct H as [n' [_ H]].
+    unfold SN0.
+    exists n'.
+    assumption.
+  -
+    unfold R; fold R.
+    split.
+    { (* Proving halting *)
+        destruct r as [r _].
+        unfold SN0 in r.
+        destruct r as [nSn r].
+        unfold SN0.
+        assert (H : exists n', n' < nSn /\ SN t' n').
+        {
+        apply forwardSN with (t := t) (t' := t') (n := nSn).
+        - exact r.
+        - assumption.  
+        }
+        destruct H as [n' [_ H]].
+        exists n'.
+        assumption.
+    }
+    intros t1 r1.
+    destruct r as [_ r].
+    specialize r with t1.
+    apply r in r1.
+    specialize IHT2 with (Ty_App t t1) (Ty_App t' t1).
+    apply IHT2 in r1.
+    + assumption.
+    + unfold RED0.
+      unfold RED0 in rd.
+      destruct rd as [s rd].
+      exists (s + 1).
+      apply RED_app1.
+      assumption. *)
+Admitted.
+
+(* R implies strongly normalizing *)
+Lemma cr1 : forall {t : tm} {tp : tp},
+    R t tp -> SN0 t.
+Proof.
+    (* intros ty K HR.
+    induction K. unfold R in HR.
+    - assumption.
+    - unfold R in HR; fold R in HR.
+      destruct HR as [sn0 _].
+      assumption. *)
+Admitted. 
+
+Lemma cr3a : forall {t t1 : tm} {tp1 tp2 : tp } {m : nat},
+  NEU t ->
+  R t1 tp1 ->
+  SN t1 m ->
+  (forall t', RED0 t t' -> R t' (tpfun tp1 tp2)) ->
+  R (tmapp t t1) tp2.
+Proof.
+  (* intros t t1 K1 K2 m neu r1 sn1 f.
+  remember (Ty_App t t1) as tt.
+  induction K2; unfold R; fold R.
+  - admit.
+  - split.
+    + admit.
+    + intros t0.  
+  destruct rd.
+  - (* Case REDapp1 *)
+    subst.
+    apply f in H.
+    apply H.
+    apply r1.
+  - (* Case REDapp2 *)
+    subst.
+    inversion sn1 as [t1' m' Hsn1].
+    specialize (Hsn1 t1' H).
+    destruct Hsn1 as [n' [Hlt Hsn1']].
+    apply cr3a with (tp1 := tp1) (tp2 := tp2) (neu := neu) (r1 := r1) (sn1 := Hsn1') (f := f).
+  - (* Case REDapp3 *)
+    subst.
+    inversion neu; subst; contradiction. *)
+Admitted.
+
+(* How do we not need kinding here... If t is a value, it is neutral, 
+  there are no t such that t --> t', so then we would have to prove R t K for all K?*)
+Lemma cr3 : forall (t : tm) (tp : tp),
+  NEU t ->
+  (forall t', RED0 t t' -> R t' tp) ->
+  R t tp.
+Proof.
+  (* intros t K neu H.
+  induction K.
+  - unfold R; fold R.
+     admit.
+      (* Suppose there is no t such that t to t', then by definition SN0 t*)
+      (* So let t' such that RED0 t t'. Then R t' Kind_Base, so SN0 t'**)
+        (* Then SN_backwards in some way. *)
+  - unfold R; fold R; split.
+    + admit. (* Same argument as above *)
+    + intros t1 Rt1.
+      remember (cr1 Rt1) as sn0.
+      unfold SN0 in sn0.
+      destruct sn0 as [sn_n sn].
+      apply (cr3a neu Rt1 sn H). *)
+Admitted. 
+
+(* Proof in Barendreght: The Lambda Calculus, 2.1.17 *)
+Lemma subst_preserves_reduction : forall t1 t2 t3 t2',
+  subst1 t1 t2 t3 ->
+  RED0 t2 t2' ->
+  exists t3', RED0 t3 t3' /\ subst1 t1 t2' t3'.
+Proof.
+Admitted.
+
+
+(* \. f  t --> subst t f t', where t' is the new term*)
+Lemma lamSN : forall (t1 t2 t3: tm) (n : nat),
+  subst1 t1 t2 t3 -> SN t3 n -> SN t2 n.
+Proof.
+(* We know that t3 normalizes in at most n steps
+    Suppose t2 steps to t2', then by subst_preserves_reduction
+    we know that t3 must also step, and then SN t3' (n - 1)
+    
+    then we do it again, but at some point we get subst1 t1 t2 t3 -> SN t3 0 -> SN t2 0
+    Proof by contradiction: Again, we suppose t2 --> t2', but it cant, because then t3 must step somewhere, and it cant.
+    So t2 cannot reduce, so it is a value, so SN t2 0. (since the implication condition is trivially true now)
+
+*)
+Admitted.
+
+(* Ask Jacco: Classical reasoning? (law of excluded middle)*)
+Lemma reduceFun :
+  forall (f t : tm) (T1 T2 : tp),
+    (R t T1 ->
+     (forall (t1 t2 : tm),
+        subst1 t1 f t2 -> R t1 T1 -> R t2 T2) ->
+     R (tmapp (tmlam f) t) T2).
+Proof.
+  (* Insight: f should have only one free variable again*)
+  intros f t T1 T2 RT1 RH.
+  specialize (RH t).
+  assert (exists t2, subst1 t f t2).
+  {
+    induction f.
+    - induction n.
+      + admit. (* t2 = t*)
+      + admit. (* Should be impossible to create, so maybe we need a well-typedness for f with only one free var?*) 
+        (* in this case, we cannot reduce though*)
+        (* So it is a value? Well.... not according to our previous value definition. 
+          a term like (\x. x y) (3) cannot reduce, but it is not a value....
+          Very problematic: is it now still a superset of our deterministic STLC?
+          *)
+  }
+  
+  
+  assert (exists n, SN f n) as SNf.
+  - admit. (* idk *)
+    (* idea: construct t2 such that subst1 t f t2*)
+    (* Then we can use it in lamSN. we need that anyway I think for using it
+       
+       What if it doesnt exist?
+       Then we cannot use REDAPP3.
+       Now suppose we reduced the f and the t
+
+       General proof idea: use backward_R (cr3) and show that all possible single step reductions work
+       For betareduce it is given by hypotheses.
+       For the others, we can go into induction, and since they are SN, we will at some point get to beta reduction
+  *)
+  
+Admitted.
+
+Lemma mainLemma :
+  forall {G : tps}  {T : tp} { ts : tms } { t t' : tm } { n : nat  },
+    DER G t T n ->
+    RS0 ts G ->
+    subst ts t t' ->
+    R t' T.
+Proof.
+  intros G T ts t t' n der rs sub.
+  generalize dependent ts.
+  generalize dependent t'.
+  induction der;
+  intros t' ts rs sub.
+  - (* Case DERvar *)
+    inversion sub.
+    apply (mainLemmaVar H H2).
+    assumption.
+  - (* Case DERlam *)
+    inversion sub.
+    unfold R; fold R.
+    intros tm' Rtm'.
+    subst...
+    apply reduceFun with  (T1 := T1); [assumption|].
+    intros t1 t2 sub1 r.
+    specialize (IHder t2).
+    pose proof (lemma20 H0 H2 sub1) as sub0.
+    specialize (IHder (tmsmore ts t1)).
+    destruct rs as [n rs_pred].
+    pose proof (RSmore rs_pred r).
+    pose proof (existT _ (S n) H) as rs.
+    specialize (IHder rs sub0).
+    assumption.
+
+  - (* Case DERapp *)
+  inversion sub.
+  specialize (IHder1 t1' ts rs H2).
+  specialize (IHder2 t2' ts rs H4).
+  unfold R in IHder1; fold R in IHder1.
+  specialize (IHder1 t2' IHder2).
+  assumption.
+Qed.
+
+(* Definition of the `reduce` lemma *)
+Lemma reduce : forall (t : tm) (T : tp),
+  DER0 tpsnil t T -> R t T.
+Proof.
+  intros t T der.
+  unfold DER0 in der.
+  remember der as der'.
+  clear Heqder'.
+  destruct der as [s der].
+  pose proof (existT _ 0 RSnil) as rs0.
+  apply (mainLemma der rs0 (lemma10 der')).
+Qed.
